work on Unfold

Pdl/Unfold.lean
@@ -2,6 +2,7 @@
 
 import Pdl.Semantics
 import Pdl.Vocab
+import Pdl.Discon
 
 -- TODO: move to Syntax.lean
 mutual
@@ -62,13 +63,72 @@ end
 
 mutual
 theorem repl_in_F_equiv x ψ :
-    (φ1 ≡ φ2) → (repl_in_F x ψ φ1) ≡ (repl_in_F x ψ φ2) := sorry
+    (φ1 ≡ φ2) → (repl_in_F x ψ φ1) ≡ (repl_in_F x ψ φ2) := sorry -- TODO easy?
 
 theorem repl_in_P_equiv x ψ :
-    (α1 ≡ᵣ α2) → (repl_in_P x ψ α1) ≡ᵣ (repl_in_P x ψ α2) := sorry
+    (α1 ≡ᵣ α2) → (repl_in_P x ψ α1) ≡ᵣ (repl_in_P x ψ α2) := sorry -- TODO easy?
 end
 
--- Lemma 45 from Yde
+
+-- ### Test Profiles
+
+-- Def 41 from Yde -- new number / name?
+
+def TestProfile (α : Program) : Type := Subtype (fun β => β ∈ testsOfProgram α) → Bool
+
+def TP (α : Program) : List (TestProfile α) := sorry
+-- TODO: generate all possible test profiles, will be finite!
+
+def signature : TestProfile α → Form := sorry
+
+theorem top_equiv_disj_TP : ⊤ ≡ dis ((TP α).map signature) := by sorry
+
+-- TODO: two more theorems here!
+
+
+
+-- Coercion of TestProfiles to subprograms
+-- These are needed to re-use `l` in the recursive calls of `F`.
+instance : CoeOut (TestProfile (α ⋓ β)) (TestProfile α) :=
+  ⟨fun l ⟨f,f_in⟩ => l ⟨f, by simp only [testsOfProgram, List.mem_union_iff]; exact Or.inl f_in⟩⟩
+instance : CoeOut (TestProfile (α ⋓ β)) (TestProfile β) :=
+  ⟨fun l ⟨f,f_in⟩ => l ⟨f, by simp only [testsOfProgram, List.mem_union_iff]; exact Or.inr f_in⟩⟩
+
+instance : CoeOut (TestProfile (α ;' β)) (TestProfile α) :=
+  ⟨fun l ⟨f,f_in⟩ => l ⟨f, by simp only [testsOfProgram, List.mem_union_iff]; exact Or.inl f_in⟩⟩
+instance : CoeOut (TestProfile (α ;' β)) (TestProfile β) :=
+  ⟨fun l ⟨f,f_in⟩ => l ⟨f, by simp only [testsOfProgram, List.mem_union_iff]; exact Or.inr f_in⟩⟩
+
+instance : CoeOut (TestProfile (∗α)) (TestProfile α) :=
+  ⟨fun l ⟨f,f_in⟩ => l ⟨f, by simp only [testsOfProgram]; exact f_in⟩⟩
+
+
+-- Def 42 from Yde -- new number / name?
+
+def F : (Σ α, TestProfile α) → List Formula
+| ⟨·_, l⟩ => ∅
+| ⟨?' τ, l⟩ => if l ⟨τ, sorry⟩ then ∅ else {~τ}
+| ⟨α ⋓ β, l⟩ => F ⟨α, l⟩ ∪ F ⟨β, l⟩
+| ⟨α;'β, l⟩ => F ⟨α, l⟩ ∪ F ⟨β, l⟩
+| ⟨∗α, l⟩ => F ⟨α, l⟩
+
+def ε : List Program := [] -- ugly way to define the empty program?
+
+def P : (Σ α, TestProfile α) → List (List Program)
+| ⟨·a, l⟩ => [ [(·a : Program)] ]
+| ⟨?' τ, l⟩ => if l ⟨τ, by simp [TestProfile,testsOfProgram] at *⟩ then ∅ else [ [] ]
+| ⟨α ⋓ β, l⟩ => P ⟨α, l⟩ ∪ P ⟨β, l⟩ -- ∪ or ++ here ??
+| ⟨α;'β, l⟩ => sorry -- TODO
+| ⟨∗α, l⟩ => [ ε ] ∪ (P (⟨α, l⟩) \ [ε]).map (fun as => as ++ [∗α])
+
+-- We use lists here because we eventually want to make formulas.
+
+def Xset (α) (l : TestProfile α) (ψ : Formula) : List Formula :=
+  F ⟨α, l⟩ ++ (P ⟨α, l⟩).map (fun as => Formula.boxes as ψ)
+
+-- TODO: def Φ_□(α,ψ) := sorry -- TODO
+
+-- Lemma 45 from Yde -- new number / name?
 theorem fortyfive (x : Char)
     (x_notin_beta : x ∉ HasVocabulary.voc β)
     (beta_equiv : (⌈β⌉·x) ≡ (((·x) ⋀ χ0) ⋁ χ1))
