Pdl/Vocab.lean
@@ -7,7 +7,7 @@ mutual
   def vocabOfProgram : Program → Finset Char
     | ·c => {c}
     | α;'β => vocabOfProgram α ∪ vocabOfProgram β
-    | Program.union α β => vocabOfProgram α ∪ vocabOfProgram β
+    | α ⋓ β => vocabOfProgram α ∪ vocabOfProgram β
     | ∗α => vocabOfProgram α
     | ?' φ => vocabOfFormula φ
   def vocabOfFormula : Formula → Finset Char
@@ -33,3 +33,21 @@ instance formulaHasVocabulary : HasVocabulary Formula := ⟨vocabOfFormula⟩
 instance programHasVocabulary : HasVocabulary Program := ⟨vocabOfProgram⟩
 instance finsetFormulaHasVocabulary : HasVocabulary (Finset Formula) := ⟨vocabOfSetFormula⟩
 instance listFormulaHasVocabulary : HasVocabulary (List Formula) := ⟨vocabOfListFormula⟩
+
+/-- Tests(α) -/
+def testsOfProgram : Program → List Formula
+| ·_ => ∅
+| ?' τ => [τ] -- no sub-tests etc. needed?
+| α;'β => testsOfProgram α ∪ testsOfProgram β
+| α ⋓ β => testsOfProgram α ∪ testsOfProgram β
+| ∗α => testsOfProgram α
+-- IDEA ? def testsOfFormula : Formula → Finset Formula
+-- class HasTests (α : Type) where testsOf : α  → Finset Formula
+
+/-- Progs(α) -/
+def subprograms : Program → List Program
+| ·a => [(·a : Program)]
+| ?' φ => [?' φ]
+| α;'β => [α;'β ] ∪ subprograms α ∪ subprograms β
+| α ⋓ β => [α ⋓ β] ∪ subprograms α ∪ subprograms β
+| ∗α => [∗α] ∪ subprograms α
